src/Rupicola/Examples/Net/IPChecksum/IPChecksum.v
@@ -36,4 +36,4 @@ Proof.
 Time Qed.
 
 Definition ip_checksum_cbytes := Eval vm_compute in
-  list_byte_of_string (ToCString.c_module [ip_checksum_br2fn]).
+  list_byte_of_string (ToCString.c_module [("ip_checksum",ip_checksum_br2fn)]).
